viper-total-heaps/CPGHelperML.thy
@@ -295,6 +295,27 @@ fun intro_fact_mask_lookup_reduction ctxt (info: basic_stmt_rel_info) exp_rel_in
   (Rmsg' "intro mask lookup red 10" (exp_rel_tac exp_rel_info ctxt) ctxt) THEN'
   (Rmsg' "intro mask lookup red 11" (assm_full_simp_solved_with_thms_tac @{thms read_mask_concrete_def} ctxt) ctxt)
 
+fun intro_fact_pred_mask_lookup_reduction ctxt (info: basic_stmt_rel_info) exp_rel_info exp_rel_perm_access_thm vpr_rcv_red_tac =
+  (Rmsg' "intro mask lookup red 1" (revcut_tac exp_rel_perm_access_thm) ctxt) THEN'
+  (Rmsg' "intro mask lookup red 2" (resolve_tac ctxt @{thms mask_read_wf_concrete} THEN'
+                                    resolve_tac ctxt [#ctxt_wf_thm info])
+                                      ctxt) THEN'
+  (Rmsg' "intro mask lookup red 4" (resolve_tac ctxt @{thms wf_ty_repr_basic}) ctxt) THEN'
+  (Rmsg' "intro mask lookup red 5" (blast_tac ctxt) ctxt) THEN'
+  (Rmsg' "intro mask lookup red 6" (vpr_rcv_red_tac ctxt |> SOLVED') ctxt) THEN'
+  (* (Rmsg' "intro mask lookup red 7" ((#field_rel_single_tac info) ctxt |> SOLVED') ctxt) THEN' *)
+  (Rmsg' "intro mask lookup" (simp_tac_with_thms [] ctxt) ctxt) THEN'
+  (* (Rmsg' "intro mask lookup red 8" (assm_full_simp_solved_with_thms_tac [#tr_def_thm info] ctxt) ctxt) THEN' *)
+  (* (Rmsg' "intro mask lookup red 9" (assm_full_simp_solved_with_thms_tac @{thms ty_repr_basic_def} ctxt) ctxt) THEN' *)
+  (Rmsg' "intro mask lookup red 10" (exp_rel_tac exp_rel_info ctxt) ctxt) THEN'
+  (Rmsg' "intro mask lookup" (simp_tac_with_thms [] ctxt) ctxt) THEN'
+  (Rmsg' "intro mask lookup" (simp_tac_with_thms [] ctxt) ctxt) THEN'
+  (Rmsg' "intro mask lookup" (simp_tac_with_thms [] ctxt) ctxt) THEN'
+  (Rmsg' "intro mask lookup" (simp_only_tac @{thms read_mask_concrete_def fun_repr_concrete.simps} ctxt) ctxt) THEN'
+  (Rmsg' "intro mask lookup" (simp_tac_with_thms [#tr_def_thm info] ctxt) ctxt) (* THEN'
+  (SUBGOAL (fn (t,_) => raise TERM ("breakpoint", [t]))) *)
+  (* (Rmsg' "intro mask lookup red 11" (assm_full_simp_solved_with_thms_tac @{thms read_mask_concrete_def} ctxt) ctxt) *)
+
 \<close>
 
 
