viper-total-heaps/ExhaleRel.thy
@@ -1096,6 +1096,7 @@ definition exhale_pred_acc_normal_premise
            exhale_pred_acc_rel_perm_success ctxt_vpr StateCons \<omega> pred_id v_args v_p \<and>
            \<omega>' = rm_from_lpm_total_full \<omega> (pred_id,v_args) (Abs_preal v_p)"
 
+
 \<comment> \<open>This rule cannot be used for the exhale in unfold, since the state relation is different.\<close>
 lemma exhale_rel_pred_acc:
   assumes WfSubexp: "exprs_wf_rel
@@ -1119,91 +1120,7 @@ lemma exhale_rel_pred_acc:
                  (\<lambda>_. False)
                  P ctxt_bpl \<gamma>\<^sub>3 \<gamma>'"
     shows "exhale_rel R R Q ctxt_vpr StateCons P ctxt_bpl (Atomic (AccPredicate pred_id e_args_vpr (PureExp e_p_vpr))) \<gamma> \<gamma>'"
-  sorry
-
-(*
-lemma exhale_rel_pred_acc_upd_rel:
-  assumes
-    StateRelIn: "\<And> \<omega>0_\<omega> ns. R \<omega>0_\<omega> ns \<Longrightarrow>
-                             state_rel Pr StateCons TyRep Tr (AuxPred(temp_perm \<mapsto> pred_eq (RealV v_p)))
-                             ctxt_bpl (fst \<omega>0_\<omega>) (snd \<omega>0_\<omega>) ns" and
-    StateRelOut: "\<And> \<omega>0_\<omega> ns. (uncurry (state_rel Pr StateCons TyRep Tr AuxPred ctxt_bpl)) \<omega>0_\<omega> ns \<Longrightarrow>
-                              R' \<omega>0_\<omega> ns" and
-    TempPermNotInAuxPred: "temp_perm \<notin> dom AuxPred" and
-
-    WfTyRep: "wf_ty_repr_bpl TyRep" and
-    MaskDefDifferent: "mask_var_def Tr \<noteq> mask_var Tr" and
-    TyInterp: "type_interp ctxt_bpl = vbpl_absval_ty TyRep" and
-
-    NullConst: "const_repr Tr CNull = nullConst" and
-    MaskVar: "m_bpl = mask_var Tr" and
-    PredLocBpl: "e_ploc_bpl = FunExp ''P'' [] [e_arg_bpl]" and
-
-    MaskUpdateWf: "mask_update_wf TyRep ctxt_bpl mask_upd_bpl" and
-    MaskReadWf: "mask_read_wf TyRep ctxt mask_read_bpl" and
-
-    NewPermBpl: "new_perm = (mask_read_bpl (Var m_bpl) (Var nullConst) e_ploc_bpl
-                                  [TConSingle ''PredicateType_P'', TPrim TBool]) \<guillemotleft>Sub\<guillemotright> (Var temp_perm)" and
-    MaskUpdateBpl: "m_upd_bpl = mask_upd_bpl (Var m_bpl) (Var nullConst) e_ploc_bpl new_perm
-                                  [TConSingle ''PredicateType_P'', TPrim TBool]" and
-
-    ArgRel: "exp_rel_vpr_bpl
-                (state_rel Pr StateCons TyRep Tr (AuxPred(temp_perm \<mapsto> pred_eq (RealV v_p))) ctxt)
-                ctxt_vpr ctxt_bpl e_arg_vpr e_arg_bpl" and
-
-    PredFunInterp: "fun_interp ctxt_bpl ''P'' = Some (lift_fun_bpl (vbpl_absval_ty TyRep) (0, [TConSingle (TRefId TyRep)], TCon (TFieldId TyRep) [TCon ''PredicateType_P'' [], TPrim TBool]) predicate_loc_P)" and
-    PredName: "pred_id = ''P''" and
-    PredLookup: "ViperLang.predicates (program_total ctxt_vpr) pred_id = Some pdecl" and
-    PredTyArgsLookup: "predicate_decl.args pdecl = ty_args" and
-    PredTyArgs: "ty_args = [TRef]"
-
-  shows "rel_general R R' 
-           (\<lambda> \<omega>0_\<omega> \<omega>0_\<omega>'. fst \<omega>0_\<omega> = fst \<omega>0_\<omega>' \<and> exhale_pred_acc_normal_premise ctxt_vpr StateCons pred_id [e_arg_vpr] e_p_vpr v_args_vpr v_p (fst \<omega>0_\<omega>) (snd \<omega>0_\<omega>) (snd \<omega>0_\<omega>'))
-           (\<lambda>_. False) P ctxt_bpl
-           (BigBlock name ((Assign m_bpl m_upd_bpl) # cs) str tr, cont)
-           (BigBlock name cs str tr, cont)"
-*)
-
-lemma exhale_rel_pred_acc_upd_rel:
-  assumes
-    StateRelIn: "\<And> \<omega> ns. R \<omega> ns \<Longrightarrow>
-                             state_rel Pr StateCons TyRep Tr (AuxPred(temp_perm \<mapsto> pred_eq (RealV v_p)))
-                             ctxt_bpl \<omega> \<omega> ns" and
-    StateRelOut: "\<And> \<omega> ns. state_rel Pr StateCons TyRep Tr AuxPred ctxt_bpl \<omega> \<omega> ns \<Longrightarrow> R' \<omega> ns" and
-    TempPermNotInAuxPred: "temp_perm \<notin> dom AuxPred" and
-
-    WfTyRep: "wf_ty_repr_bpl TyRep" and
-    (* MaskDefDifferent: "mask_var_def Tr \<noteq> mask_var Tr" and *)
-    TyInterp: "type_interp ctxt_bpl = vbpl_absval_ty TyRep" and
-
-    NullConst: "const_repr Tr CNull = nullConst" and
-    MaskVar: "m_bpl = mask_var Tr" and
-    PredLocBpl: "e_ploc_bpl = FunExp ''P'' [] [e_arg_bpl]" and
-
-    MaskUpdateWf: "mask_update_wf TyRep ctxt_bpl mask_upd_bpl" and
-    MaskReadWf: "mask_read_wf TyRep ctxt mask_read_bpl" and
-
-    MaskUpdateBpl: "m_upd_bpl = mask_upd_bpl (Var m_bpl) (Var nullConst) e_ploc_bpl new_perm
-                                  [TConSingle ''PredicateType_P'', TPrim TBool]" and
-    NewPermBpl: "new_perm = (mask_read_bpl (Var m_bpl) (Var nullConst) e_ploc_bpl
-                                  [TConSingle ''PredicateType_P'', TPrim TBool]) \<guillemotleft>Sub\<guillemotright> (Var temp_perm)" and
-
-    ArgRel: "exp_rel_vpr_bpl
-                (state_rel Pr StateCons TyRep Tr (AuxPred(temp_perm \<mapsto> pred_eq (RealV v_p))) ctxt)
-                ctxt_vpr ctxt_bpl e_arg_vpr e_arg_bpl" and
-
-    PredFunInterp: "fun_interp ctxt_bpl ''P'' = Some (lift_fun_bpl (vbpl_absval_ty TyRep) (0, [TConSingle (TRefId TyRep)], TCon (TFieldId TyRep) [TCon ''PredicateType_P'' [], TPrim TBool]) predicate_loc_P)" and
-    PredName: "pred_id = ''P''" and
-    PredLookup: "ViperLang.predicates (program_total ctxt_vpr) pred_id = Some pdecl" and
-    PredTyArgsLookup: "predicate_decl.args pdecl = ty_args" and
-    PredTyArgs: "ty_args = [TRef]"
-
-  shows "rel_general R R'
-           (\<lambda> \<omega> \<omega>'. exhale_pred_acc_normal_premise ctxt_vpr StateCons pred_id [e_arg_vpr] e_p_vpr v_args_vpr v_p \<omega> \<omega> \<omega>')
-           (\<lambda>_. False) P ctxt_bpl
-           (BigBlock name ((Assign m_bpl m_upd_bpl) # cs) str tr, cont)
-           (BigBlock name cs str tr, cont)"
-  sorry
+  oops
 
 
 subsection \<open>Misc\<close>
